\documentclass{article}

\input{../../header.tex}

\title{Math 1540: HW1}

\begin{document}

\maketitle
\emph{Book Problems:}
\begin{enumerate}
    \item[49.] This is equivalent to proving that a polynomial \(p(x) \in F[x]\) of degree 2 or 3 must have at least one root in \(F\)  iff \(p(x)\) is reducible
    
    Suppose there exists a root, \(a\), in \(F\) then a linear term \((x - a)\) can be divided out from \(p(x)\) (Euclidean division); therefore \(p(x)\) is reducible
    
    Suppose \(p(x)\) is reducible, then \(p(x)\) can be written as \(p(x) = f(x)g(x)\) where \(deg(f(x))\) and \(deg(g(x))\) are not equal to \(0\). \(deg(p(x)) = deg(f(x)) + deg(g(x))\) In the case of \(deg(p(x))= 2\), \(deg(f(x))\) must be less than 2 and not equal to 0, so it's a linear term, and so \(p(x)\) has a root in \(F\). In the case of \(deg(p(x))= 3\), either \(deg(f(x))\) or \(deg(g(x))\) must be less than 2 and not equal to 0, so either \(f(x)\) or \(g(x)\) is a linear term, and so \(p(x)\) has a root in \(F\).

    \item[50.] Since \(p(x) \in F[x]\) is irreducible \(p(x)\) is a maximal ideal therefore either \(g(x) \in (p(x)) \iff p(x)|g(x)\) or \(g(x) \notin (p(x)) \iff (p(x), g(x))\) contains the entire ring \(\iff (p(x), g(x))\) = 1

    \item[63.] Let the monic polynomial \(f(x) = a_0 + a_1 x \ldots a_n x^n\) where \(a_n = 1\) then \(s | 1 \implies s = 1\) and \(r \in \Z\); therefore \(r/s = r\) is an integer

    \item[69.] Using the rational root thm and the fact that this polynomial (degree 3) has a root in \(\Z\) (from Q49). \(1,36,2,18,3,12,4,9,6\) all could be roots. By calculation, we can see that 3 is a root (\(3^3 + 3^2 - 36 = 0\)). Using Euclidean division we find that \(x^3 + x^2 - 36\) splits into \((x-3)(x^2 + 4x - 12)\) Now we must check whether \((x^2 + 4x + 12)\) factors and using the discriminant from the Quadratic formula \(b^2 - 4ac\) we find the discriminant is negative \(16 - 4(1)(12)\), so \((x^2 + 4x + 12)\) cannot be factored further in \(\Q[x]\)  
\end{enumerate}

\emph{Given Problems:}
\begin{enumerate}
    \item[1.] Let \(a = y^3\), then \(y^6 + ry^3 - q^3 / 27\) becomes \(a^2 + ra - q^3 / 27\). Now it is clear that this is in the form of a quadratic and we can solve it using the Quadratic formula. Therefore, \(a = y^3 = (-r \pm \sqrt{r^2 + 4q^3 / 27})/2\) 
    
    \emph{Note: Like in the question I will be using the same notation (variables) as in the textbook. Some of the formulas/equations I use will be from the textbook (Rotman).}

    From page 45 in the textbook we see that \(y^3 z^3 = -q^3 / 27\). From page 46 in the textbook we see that the roots are given as \(y+z, wy + w^2 z, w^2 y +wz\)

    Throughout the entire derivation of the cubic formula in the textbook both \(y\) and \(z\) are interchangeable (there is a symmetry between the two variables)
    
    Let \(y_1 = y^3 =\frac{1}{2}\left(-r + \sqrt{r^2+4 q^3 / 27}\right)\) and \(y_2 = y^3 =\frac{1}{2}\left(-r - \sqrt{r^2+4 q^3 / 27}\right)\) 

    Then
    \begin{eqnarray*}
        y_1y_2 =
        \frac{1}{4}(r^2 - (r^2 + 4q^3 / 27)) =
        \frac{1}{4}(-  4q^3 / 27) =
        - q^3 / 27
    \end{eqnarray*}

    This mirrors an earlier result \(y^3 z^3 = -q^3 / 27\), and suggests that if \(y^3 =\frac{1}{2}\left(-r + \sqrt{r^2+4 q^3 / 27}\right)\) then \(z^3 =\frac{1}{2}\left(-r - \sqrt{r^2+4 q^3 / 27}\right)\) and vice versa. And so, because of the symmetry of the variables \(y\) and \(z\) the choice between the \(+\) and \(-\) does not matter.

    \item[2.] Let the characteristic, \(q = mn \neq 0\), of a field, \(F\), be composite, then \(m1_F \cdot n1_F = q1_F = 0\) but \(m1_F, n1_F \neq 0\); this is a contradiction since this implies that \(m1_f\) and \(n1_F\) are zero divisors, yet are in a field \(F\)
 
    \item[3.] Case \(n = 0\):
    Consider the map \(f: \Z \to F\) such that \(f(m) = m1_F\).
    This map is a homomorphism since:
    \begin{eqnarray*}
        f(m + p) =
        (m + p)1_F =
        m1_F + p1_F =
        f(m) + f(p)
    \end{eqnarray*}
    \begin{eqnarray*}
        f(mp) =
        (mp)1_F =
        m1_F \cdot n1_F =
        f(m) \cdot f(n)
    \end{eqnarray*}
     Using this map we can construct a map to the \(\Q\) similar to how we can create \(\Q\) from \(\Z\) 
    
    Consider the map \(g: \Q \to F\) such that \(g(m/p) = f(m)/f(p)\) with \(p \neq 0\) (to clarify \(m, p \in \Z\) so \(m/p \in \Q\)) This map is a homomorphism since 
    \begin{eqnarray*}
        g(\frac{m_1}{p_1} \cdot \frac{m_2}{p_2}) =
        g(\frac{m_1m_2}{p_1p_2}) =
        (\frac{f(m_1)f(m_2)}{f(p_1)f(p_2)}) =
        (\frac{f(m_1)}{f(p_1)} \cdot \frac{f(m_2)}{f(p_2)}) =
        g(\frac{m_1}{p_1}) \cdot g(\frac{m_2}{p_2})
    \end{eqnarray*}
    \begin{eqnarray*}
        g(\frac{m_1}{p_1} + \frac{m_2}{p_2}) =
        g(\frac{m_1 + m_2}{p_1 + p_2}) =
        (\frac{f(m_1) + f(m_2)}{f(p_1) + f(p_2)}) =
        (\frac{f(m_1)}{f(p_1)} \cdot \frac{f(m_2)}{f(p_2)}) =
        g(\frac{m_1}{p_1}) + g(\frac{m_2}{p_2})
    \end{eqnarray*}

    Since any homomorphism between two fields is injective, this map is an injective map from \(\Q\) to \(F\). Therefore, F contains a subfield isomorphic to image of \(g\), which in this case is \(\Q\). Since the image is in terms of \(1_F\) all fields must contain the image of \(g\) and the image of \(g\) is a subfield, so it must be \(P\)  

    Case \(n = p\):
    When \(n = p\) the image of \(g\) is \(\{0, 1_F \ldots (p-1)1_F \}\) Therefore, \(\Z_p\) is isomorphic to \(P\)    

    \item[4.] We showed in Q63 that if we have a monic polynomial, in this case \(p(x)\), the rational root must be an integer; moreover, since the leading coefficient is 1 (\(s\) must be 1) we know that the rational root \(r/s = r\), and by the rational root thm, \(r | a_0 = 30\). The possible rational roots are \(1,30,2,15,3,10,5,6\). By calculation, can see that \(2\) is a root \(2^3 - 19 + 30\). Using Euclidean division we find that \(x^3 - 19 x + 30\) splits into \((x-2)(x^2 + 2x - 15)\). We know the sum of the other two roots must be \(-2\), the negative of the linear coefficient of \((x^2 + 2x - 15)\) (Note: \((x-a)(x-b) = x^2 - (a+b)x  + ab\) so negative of the linear term is the sum of the roots); therefore, the sum of all the roots is \(s_1 + s_2 + s_3 = 0\).

    In the question, "expression," was somewhat vague so if it meant \(s_1\): by factoring \((x^2 + 2x - 15) = (x + 5)(x - 3)\) (or using the Quadratic formula) we find that \(-5, 3\) are the remaining roots. Since \(-5, 2, 3\) divide \(30\), \(s_1\) divides \(30\). \(s_1 = 3\)     
\end{enumerate}

\end{document}